fixing an unfolding issue

src/typechecker/rel.fs
@@ -318,11 +318,11 @@ let base_and_refinement env wl t1 =
         | Tm_app _ ->
             if norm
             then (t1, None)
-            else let t2', refinement = aux true (normalize_refinement [N.WHNF;N.UnfoldUntil Delta_constant] env wl t1) in
-                 begin match refinement with
-                    | None -> t1, None (* no refinement found ... so revert to the original type, without expanding defs *)
-                    | _ -> t2', refinement
-                 end
+            else let t1' = normalize_refinement [N.WHNF;N.UnfoldUntil Delta_constant] env wl t1 in
+                 begin match (SS.compress t1').n with 
+                            | Tm_refine _ -> aux true t1'
+                            | _ -> t1, None
+                   end
 
         | Tm_type _
         | Tm_constant _
